DNFP and some rewrite
Rewrote lemmas/proofs of pair monad and started DNFP

Monad_Play Around/Int_Pair_State_Fib.thy
@@ -17,6 +17,19 @@ definition put_fst:: "'a \<Rightarrow> ('a pair, unit) state" where "put_fst x =
 definition put_snd:: "'a \<Rightarrow> ('a pair, unit) state" where "put_snd x = do { v \<leftarrow> get; put (set_snd v x) }"
 definition skip:: "('a pair, unit) state" where "skip = State (\<lambda>x. ((),x))"
 
+(*
+definition return:: "nat \<Rightarrow> ('b, nat) state" where "return = State_Monad.return"
+definition get:: "(nat pair, nat pair) state" where "get = State (\<lambda>x. (x,x))"
+definition put:: "nat pair \<Rightarrow> (nat pair, unit) state" where "put x = State (\<lambda>_. ((),x))"
+definition get_fst:: "(nat pair, nat) state" where "get_fst = do { x \<leftarrow> get; return (fst x) }"
+definition get_snd:: "(nat pair, nat) state" where "get_snd = do { x \<leftarrow> get; return (snd x) }"
+definition set_fst:: "nat pair \<Rightarrow> nat \<Rightarrow> nat pair" where "set_fst v x = (x, snd v)"
+definition set_snd:: "nat pair \<Rightarrow> nat \<Rightarrow> nat pair" where "set_snd v x = (fst v, x)"
+definition put_fst:: "nat \<Rightarrow> (nat pair, unit) state" where "put_fst x = do { v \<leftarrow> get; put (set_fst v x) }"
+definition put_snd:: "nat \<Rightarrow> (nat pair, unit) state" where "put_snd x = do { v \<leftarrow> get; put (set_snd v x) }"
+definition skip:: "(nat pair, unit) state" where "skip = State (\<lambda>x. ((),x))"
+*)
+
 fun fibacc :: "nat \<Rightarrow> nat => nat \<Rightarrow> nat" where
 fa1: "fibacc 0 a b = a"| 
 fa2: "fibacc (Suc 0) a b = b"|
@@ -48,8 +61,7 @@ lemma fib_aux: "fibacc n b (a + b) = fibacc (Suc n) a b"
 
 lemma fib_aux1: "fibacc (Suc (Suc n)) a b = fibacc n a b + fibacc (Suc n) a b"
   apply(induct n arbitrary: a b)
-  apply(simp)
-  apply(simp)
+  apply(simp_all)
   apply(simp only: fib_aux)
   done
 
@@ -74,55 +86,41 @@ text\<open>The fibonacci function does always return the result at the fst value
 fun monfib:: "nat \<Rightarrow> (nat pair, unit) state" where
   "monfib 0 = skip" |
   "monfib (Suc 0) = do {b \<leftarrow> get_snd; put_fst b}" |
-  "monfib (Suc (Suc n)) = do { a \<leftarrow> get_fst; b \<leftarrow> get_snd; temp_b \<leftarrow> return b; b \<leftarrow> return (a + b); put (temp_b,b); monfib (Suc n)}"
+  "monfib (Suc (Suc n)) = do { a \<leftarrow> get_fst; b \<leftarrow> get_snd; put (b,(a + b)); monfib (Suc n)}"
 
 text\<open>Stefan do you - know why I can't run any of these examples?\<close>
 value \<open>fst(snd(run_state (monfib 5) (fst((0,1), ()))))\<close>
+value \<open>fst(snd(run_state (monfib 5) (0,1)))\<close>
+
 value "fst(snd (run_state (monfib 6) x))"
 
 lemma monfib_aux: "fst(snd (run_state (monfib n) (b, (a + b)))) = fst(snd (run_state (monfib (Suc n)) (a, b)))"
-  apply(simp_all only: skip_def snd_def fst_def get_fst_def get_snd_def put_def put_fst_def return_def get_def)
   apply(induction n rule: nat.induct)
-   apply(simp)
-   apply(simp only: skip_def snd_def fst_def get_fst_def get_snd_def put_def put_fst_def get_def return_def set_fst_def)
-   apply(simp add: get_snd_def return_def put_def get_fst_def get_def)
-  apply(simp add: get_fst_def return_def get_snd_def put_def get_def)
-done
+   apply(simp_all add: skip_def snd_def fst_def get_fst_def get_snd_def put_def put_fst_def get_def return_def set_fst_def)
+  done
 
 value "fst(snd (run_state (monfib (Suc (Suc 4))) x)) 
         = fst(snd (run_state (monfib 4) x)) + fst(snd (run_state (monfib (Suc 4)) x))"
 
 lemma monfib_aux1: "fst(snd (run_state (monfib (Suc (Suc n))) x)) 
       = fst(snd (run_state (monfib n) x)) + fst(snd (run_state (monfib (Suc n)) x))"
-  apply(simp_all add: skip_def snd_def fst_def get_fst_def get_snd_def put_def put_fst_def return_def get_def)
   apply (induction n arbitrary: x rule: nat.induct)
-   apply (simp)
-   apply (simp only: skip_def get_snd_def return_def snd_def get_def put_fst_def set_fst_def put_def get_fst_def fst_def)
-   apply (simp add: return_def)
-   apply (simp)
-   apply (simp only: skip_def get_snd_def return_def snd_def get_def put_fst_def set_fst_def put_def get_fst_def fst_def)
-  apply (simp)
+   apply (simp_all add: skip_def get_snd_def return_def snd_def get_def put_fst_def set_fst_def put_def get_fst_def fst_def)
   by (simp add: case_prod_beta' monfib_aux)
 
 lemma fib_mon_basic: "fst(snd(run_state (monfib n) (a,b))) = fibacc n a b"
-  apply(simp_all add: skip_def snd_def fst_def get_fst_def get_snd_def put_def put_fst_def return_def get_def)
   apply (induction n arbitrary: a b)
-   apply (simp_all add: skip_def)
+  apply(simp_all add: skip_def snd_def fst_def get_fst_def get_snd_def put_def put_fst_def)
   by (metis case_prod_beta' fib_aux monfib_aux)
 
 lemma fib_m_main: "fst(snd(run_state (monfib n) (0,1))) = fib n"
   apply (induction n rule:fib.induct)
-    apply(simp add: snd_def put_def get_def return_def skip_def fst_def)
-    apply(simp add: snd_def put_def get_def return_def skip_def fst_def put_fst_def get_snd_def set_fst_def)
-  apply(simp add: snd_def get_fst_def get_def get_snd_def return_def fst_def put_def)
+  apply(simp_all add: skip_def snd_def fst_def get_fst_def get_snd_def put_def put_fst_def get_def return_def set_fst_def)
   by (metis One_nat_def add.commute case_prod_beta' monfib_aux monfib_aux1 plus_1_eq_Suc)
 
 lemma fib_basic_aux: "fst(snd(run_state (monfib n) (0,1))) = fibacc n 0 1"
-  apply(simp_all add: skip_def snd_def fst_def get_fst_def get_snd_def put_def put_fst_def return_def get_def)
-  apply (induction n)
-   apply (simp add: skip_def)
+apply (induction n)
+apply(simp_all add: skip_def snd_def fst_def)
   by (metis One_nat_def case_prod_beta' fib_m_main fib_main1)
-
-
 
 end
