Monad_Play Around/Dutch_National_Flag.thy
@@ -1,0 +1,44 @@
+theory Dutch_National_Flag
+imports 
+  Main
+  "~~/src/HOL/Library/State_Monad"
+
+begin
+definition swap:: "'a list \<Rightarrow> nat \<Rightarrow> nat \<Rightarrow> 'a list" where
+"swap xs i j \<equiv> (if i < length xs \<and> j < length xs then xs[i := xs!j, j := xs!i] else xs)"
+
+lemma length_swap[simp]: "length(swap xs i j) = length xs"
+  by(simp add: swap_def)
+
+lemma distinct_swap[simp]:
+  "distinct(swap xs i j) = distinct xs"
+  by(simp add: swap_def)
+
+value\<open>swap [a,b,c,d,e] 0 4 = [e,b,c,d,a]\<close>
+
+
+(*How to loo up in a list*)
+fun dnfp:: "nat list \<Rightarrow> nat list \<Rightarrow> nat \<Rightarrow> nat \<Rightarrow> nat \<Rightarrow> nat \<Rightarrow> nat list" where
+"dnfp [] s _ _ _ _ = s"|
+"dnfp (x#xs) s low high i mid = (if high > i then (if s!i < mid then (dnfp xs (swap s i low) (Suc low) high (Suc i) mid)
+                                  else (if s!i > mid then (dnfp xs (swap s i high) low (high-1) (Suc i) mid)
+                                        else (dnfp xs s low high (Suc i) mid))) else s)"
+
+
+text\<open>How do I evaluate this - where I define a variable/constant and use it in a function call\<close>
+value\<open>\<lbrakk>xs = [0,0,2,2,1]\<rbrakk> \<Longrightarrow> (dnfp xs xs 0 4 0 1) = [0,0,1,2,2]\<close>
+value\<open>(dnfp [0,0,2,2,1] [0,0,2,2,1] 0 4 0 1) = [0,0,1,2,2]\<close>
+value\<open>(dnfp [1,0,2,0,2,0,2,1] [1,0,2,0,2,0,2,1] 0 8 0 1) = [0,0,0,1,1,2,2,2]\<close>
+value\<open>(dnfp [1,0,2,0,2,0,2,1] [1,0,2,0,2,0,2,1] 0 8 0 1)\<close>
+value\<open>(dnfp [1,0,2,0,2,0,2,1] [1,0,2,0,2,0,2,1] 0 8 0 1)\<close>
+
+value\<open>(dnfp [1,0,2,0,2,2,1] [1,0,2,0,2,2,1] 0 6 0 1)\<close>
+
+value\<open>sorted(dnfp [1,0,2,0,2,0,2,1] [1,0,2,0,2,0,2,1] 0 8 0 1)\<close>
+value\<open>sorted(dnfp [1,0,2,0,2,2,1] [1,0,2,0,2,2,1] 0 7 0 1)\<close>
+value\<open>sorted(dnfp [1,0,2,0,2,2,1,0] [1,0,2,0,2,2,1,0] 0 7 0 1)\<close>
+value\<open>(dnfp [1,0,2,0,2,2,1,0] [1,0,2,0,2,2,1,0] 0 7 0 1)\<close>
+
+
+
+end
